theories/clang/ret_logic.v
@@ -11,21 +11,18 @@ Section wp_ret.
   (* local case *)
   (∃ eh K,
      ⌜to_val e1 = None ∧ unfill_expr e1 [] = Some (K, eh) ⌝ ∧
-     ((⌜ is_jmp eh = false ⌝ ∗ WP eh @ E {{ v, ▷ wpr E (fill_ectxs (Evalue v) K) Φ Φret }}) ∨
-      (⌜ is_jmp eh = true ⌝ ∗ WP eh @ E {{ Φret }}))
+     ((⌜ is_jmp eh = false ⌝ ∗ WP eh @ E {{ v, wpr E (fill_ectxs (Evalue v) K) Φ Φret }}) ∨
+      (∃ v, ⌜ eh = Erete (Evalue v) ⌝ ∗ (stack_interp [[]] -∗ WP (Evalue v) @ E {{ Φret }})) ∨
+      (∃ f ls, ⌜ eh = Ecall f (map (λ l : addr, Evalue (Vptr l)) ls) ⌝ ∗
+               (stack_interp [[]] -∗
+                WP eh @ E {{ v, ▷ wpr E (fill_ectxs (Evalue v) K) Φ Φret }})))
   ))%I.
 
-  Local Instance wp_pre_contractive : Contractive wp_pre.
-  Proof. 
-    rewrite /wp_pre=> n wp wp' Hwp E e1 Φ.
-    repeat (f_contractive || f_equiv); apply Hwp.
-  Qed.
-  
   Local Instance wpr_pre_contractive : Contractive wpr_pre.
-  Proof.
+  Proof.    
     rewrite /wpr_pre=> n wp wp' Hwp E e1 Φ Φret.
-    repeat (f_contractive || f_equiv); apply Hwp.
-  Qed.
+    (* repeat (f_contractive || f_equiv); apply Hwp. *)
+  Admitted.
   
   Definition wpr_def:
   coPset → expr → (val → iProp Σ) → (val → iProp Σ) → iProp Σ := fixpoint wpr_pre.
@@ -36,6 +33,22 @@ Section wp_ret.
   Lemma wpr_unfold E e Φ Φret : wpr E e Φ Φret ⊣⊢ wpr_pre wpr E e Φ Φret.
   Proof. rewrite wpr_eq. apply (fixpoint_unfold wpr_pre). Qed.
 
+  Lemma wpr_helper E P R Q e eh K:
+    unfill_expr e [] = Some (K, eh) →
+    (∀ v, P v ∗ R ⊢ Q v) →
+    ▷ R ∗
+    WP eh @ E {{ P }}
+    ⊢ WP eh @ E {{ Q }}.
+  Proof.
+    iIntros (??) "[HR ?]".
+    assert (to_val eh = None) as ?; first admit.
+    iDestruct (wp_frame_step_l' with "[-]") as "?"=>//.
+    { iFrame "HR". iFrame. }
+    iApply (wp_strong_mono E E)=>//.
+    iFrame. iIntros (?) "[? ?]".
+    iModIntro. iApply H1. iFrame.
+  Admitted.
+    
   Lemma wpr_bind kes E e Φ Φret :
     wpr E e (fun v => wpr E (fill_ectxs (Evalue v) kes) Φ Φret) Φret
     ⊢ wpr E (fill_ectxs e kes) Φ Φret.
@@ -45,23 +58,94 @@ Section wp_ret.
     - iDestruct "H" as (v) "[% ?]".
       apply of_to_val in H0. subst.
       by rewrite wpr_unfold /wpr_pre.
-    - iDestruct "H" as (eh K) "(% & [[% ?] | [% ?]])"; destruct H0.
+    - iDestruct "H" as (eh K) "(% & [[% ?]| [? | ?]])"; destruct H0.
       + iRight. iExists eh, (kes ++ K).
         iSplit.
         * iPureIntro. split.
           { by apply fill_ectxs_not_val. }
           { by apply unfill_app. }
         * iLeft. iSplitL ""; first done.
-          iApply (wp_strong_mono E E _ _ _)=>//.
-          iFrame. iIntros (?) "?".
-          iModIntro. iNext.
-          iSpecialize ("IH" $! E (fill_ectxs (Evalue a) K) Φ Φret).
-          rewrite fill_app. by iApply "IH".
-      + iRight. iExists eh, (kes ++ K). iSplit.
+          iApply wpr_helper=>//; last (iFrame "IH"; iFrame).
+          iIntros (?) "[? ?]".
+          iSpecialize ("~1" $! E (fill_ectxs (Evalue _) K) Φ Φret).
+          rewrite fill_app. by iApply "~1".
+      + iDestruct "~" as (v) "[% ?]". iRight. iExists eh, (kes ++ K). iSplit.
         * iPureIntro. split.
           { by apply fill_ectxs_not_val. }
           { by apply unfill_app. }
-        * iRight. by iSplitL "".
+        * iRight. iLeft. iExists v. by iSplitL "".
+      + iDestruct "~" as (??) "[% ?]".
+        iRight. iExists eh, (kes ++ K). iSplit.
+        * iPureIntro. split.
+          { by apply fill_ectxs_not_val. }
+          { by apply unfill_app. }
+        * iRight. iRight. iExists H2, H3.
+          iSplitL ""; first done. iIntros "?".
+          iDestruct ("~1" with "~") as "?".
+          iApply (wp_strong_mono E E)=>//.
+          iFrame. iIntros (?) "?".
+          iModIntro. iNext.
+          iSpecialize ("IH" $! E (fill_ectxs (Evalue a) K)).
+          rewrite fill_app. by iApply "IH".
+  Qed.
+
+  Lemma wpr_ret v E Φ Φret:
+    Φret v ⊢ wpr E (Erete (Evalue v)) Φ Φret.
+  Proof.
+    iIntros "H".
+    rewrite wpr_unfold /wpr_pre.
+    iRight. iExists (Erete (Evalue v)), [].
+    iSplit.
+    - iPureIntro. split=>//.
+    - iRight. iLeft. iExists v. iSplitL ""; first done.
+      iIntros "?".
+      by iApply wp_value.
   Qed.
   
+  Lemma wp_something E e Φ:
+    wpr E e (λ _ : val, False) Φ
+    ⊢ WP e @ E {{ v, Φ v }}.
+  Proof.
+    iIntros "H". iLöb as "IH" forall (E e Φ). rewrite !wpr_unfold /wp_pre.
+    iDestruct "H" as "[H | H]".
+    - by iDestruct "H" as (v) "[_ %]".
+    - iDestruct "H" as (eh K) "(% & [[% ?]| [? | ?]])"; destruct H0.
+      + assert (e = fill_ectxs eh K) as ?; first admit.
+        subst. iApply wp_bind=>//.
+        iApply wpr_helper=>//; last (iFrame "IH"; iFrame).
+        iIntros (v) "[? IH]".
+        by iApply "IH".
+      + iDestruct "~" as (v) "[% ?]".
+        subst. assert (e = fill_ectxs (Erete (Evalue v)) K) as ?; first admit.
+        subst. iApply (wp_ret _ [] [[]]).
+        iSplitL ""; first admit.
+        iIntros "?".
+        simpl. by iDestruct ("~1" with "~") as "?".
+      + iDestruct "~" as (f ls) "[% ?]".
+        assert (e = fill_ectxs eh K) as ?; first admit. subst.
+        iAssert (stack_interp [[]]) as "H"; first admit.
+        iDestruct ("~1" with "H") as "?".
+        admit.
+  Admitted.
+  
+  Lemma wpr_call E es ls params f_body f_body' f retty Φ Φret:
+    es = map (fun l => Evalue (Vptr l)) ls →
+    instantiate_f_body (add_params_to_env (Env [] []) params ls) f_body = Some f_body' →
+    text_interp f (Function retty params f_body) ∗
+    ▷ wpr E f_body' (fun _ => False%I) Φ
+    ⊢ wpr E (Ecall f es) Φ Φret.
+  Proof.
+    iIntros (??) "[? ?]".
+    iApply wpr_unfold. rewrite /wpr_pre.
+    iRight. iExists (Ecall f es), [].
+    iSplit.
+    { iPureIntro. split=>//. simpl.
+      subst. by rewrite forall_is_val. }
+    iRight. iRight. iExists f, ls. subst. iSplitL ""; first done.
+    iIntros "?".
+    iApply (wp_call _ [])=>//.
+    iFrame. iNext. iIntros "?".
+    simpl. iApply wp_something.
+  Admitted.
+    
 End wp_ret.
